WIP: move back and revive Hyperproperties file

io/Hyperproperties.fst
@@ -9,13 +9,13 @@ open FStar.String
 open FStar.Tactics
 open FStar.List.Tot
 
-open IIO
-open IIO.Behavior
+open MIO
+open MIO.Behavior
 open BeyondCriteria
 open Compiler.Model
 
 (** this is a second definition of reify that is in the Tot effect **)
-assume val _tot_reify_IIOwp (#a:Type) (#wp:Hist.hist a) (#fl:erased tflag) ($f:unit -> IIOwp a fl wp) : Tot (dm_giio a fl wp)
+assume val _tot_reify_MIOwp (#a:Type) (#wp:Hist.hist a) (#fl:erased tflag) ($f:unit -> MIOwp a fl wp) : Tot (dm_gmio a fl wp)
 
 (** ** Non-interference theorems for ctx **)
 (* Termination-insensitive noninterference (TINI) definition took from Beyond Full Abstraction
@@ -47,18 +47,18 @@ h2 = [EOpenfile;Eopenfile]  lt2 = []                 r2 = 42
 let make_rc_tree (#a:Type) (#b:Type) (rc:rc_typ a b) : tree pck_rc =
   Node (| a, b, rc |) Leaf Leaf
 
-type event_dtuple = (cmd:io_cmds & (arg:io_sig.args cmd) & io_sig.res cmd arg)
+type event_dtuple = (bool & cmd:io_cmds & (arg:io_sig.args cmd) & io_sig.res cmd arg)
 val (!) : event -> event_dtuple
 let (!) = destruct_event
 
 (** the context can learn more things after it does IO actions **)
-let hist_public_inputs (pi:monitorable_prop) (rc:rc_typ 'a 'b) (h1 h2 ctx_lt:trace) : Type0 =
+let hist_public_inputs (#pi:policy_spec) (phi:policy pi) (rc:rc_typ 'a 'b) (h1 h2 ctx_lt:trace) : Type0 =
   (* TODO: there is no need to write forall cmds. one can restrict it for the heads of the two traces *)
-  (forall cmd arg. pi cmd arg (rev ctx_lt @ h1) == pi cmd arg (rev ctx_lt @ h2)) /\
+  (forall cmd arg. phi (rev ctx_lt @ h1) cmd arg == phi (rev ctx_lt @ h2) cmd arg) /\
   (** the runtime checks can be partially applied, so we have to
       take in consideration when were they first partially applied
       and when were they completely applied. The ctx has access to 
-      effectful runtime checks of type: eff_rc_typ = 'a -> 'b -> IIO bool **)
+      effectful runtime checks of type: eff_rc_typ = 'a -> 'b -> MIO bool **)
   (forall (i:nat) x y. i < length ctx_lt ==> (
     let call1, call2 = splitAt i ctx_lt in
     rc x (rev call1 @ h1) y call2 == rc x (rev call1 @ h2) y call2))
@@ -66,24 +66,24 @@ let hist_public_inputs (pi:monitorable_prop) (rc:rc_typ 'a 'b) (h1 h2 ctx_lt:tra
 (** the call of an IO action is an output 
     from the context to the environment **)
 let ctx_output (e:event_dtuple) : cmd:io_cmds & io_sig.args cmd =
-  let (| cmd, arg, _ |) = e in
+  let (| _, cmd, arg, _ |) = e in
   (| cmd, arg |)
 
 (** the result of an IO action is an input
     from the environment to the context **)
-let env_input (e:event_dtuple) : io_sig.res (Mkdtuple3?._1 e) (Mkdtuple3?._2 e) =
-  let (| cmd, arg, res |) = e in
+let env_input (e:event_dtuple) : io_sig.res (Mkdtuple4?._2 e) (Mkdtuple4?._3 e) =
+  let (| _, cmd, arg, res |) = e in
   res
 
-let rec ni_traces (pi:monitorable_prop) (rc:rc_typ 'a 'b) (r1 r2:int) (h1 h2 acc_lt lt1 lt2:trace) : 
+let rec ni_traces (pi:policy_spec) (phi:policy pi) (rc:rc_typ 'a 'b) (r1 r2:int) (h1 h2 acc_lt lt1 lt2:trace) : 
   GTot Type0 (decreases lt1) =
-  hist_public_inputs pi rc h1 h2 acc_lt ==> (
+  hist_public_inputs phi rc h1 h2 acc_lt ==> (
     match lt1, lt2 with
     | [], [] -> r1 == r2
     | hd1::t1, hd2::t2 -> begin
         (ctx_output !hd1 == ctx_output !hd2 /\
         (** determinacy **)
-        (env_input !hd1 == env_input !hd2 ==> ni_traces pi rc r1 r2 h1 h2 (acc_lt@[hd1]) t1 t2))
+        (env_input !hd1 == env_input !hd2 ==> ni_traces pi phi rc r1 r2 h1 h2 (acc_lt@[hd1]) t1 t2))
     end
     | _, _ -> False)
 
@@ -95,134 +95,134 @@ TODO:
 - [ ] prove 
 *)
 val ni : 
-  pi : monitorable_prop ->
+  pi : policy_spec ->
+  phi : policy pi ->
   (** for any runtime check **)
   rc : (rc_typ 'a 'b) ->
   (** the ctx is in a first-order setting. I don't think it matters **)
-  ctx: (fl:erased tflag -> pi:erased monitorable_prop -> typ_io_cmds fl pi -> typ_eff_rcs fl (make_rc_tree rc) -> unit -> IIO int fl (fun _ -> True) (fun _ _ _ -> True)) ->
+  ctx: (fl:erased tflag -> pi:erased policy_spec -> acts fl pi false -> typ_eff_rcs fl (make_rc_tree rc) -> unit -> MIO int fl (fun _ -> True) (fun _ _ _ -> True)) ->
   Lemma (
                                   (** one has to instantiate the ctx to be able to call beh **)
-    let bh = beh_ctx #(fun _ -> True) (ctx AllActions pi (inst_io_cmds pi) (make_rcs_eff (make_rc_tree rc))) in
+    let bh = beh_ctx #(fun _ -> True) (ctx AllActions pi (inst_io_cmds phi) (make_rcs_eff (make_rc_tree rc))) in
     forall h1 lt1 r1 h2 lt2 r2. 
       (h1, Finite_trace lt1 r1) `pt_mem` bh /\ 
       (h2, Finite_trace lt2 r2) `pt_mem` bh ==> 
-      ni_traces pi rc r1 r2 h1 h2 [] lt1 lt2)
+      ni_traces pi phi rc r1 r2 h1 h2 [] lt1 lt2)
 
 // parametricity ==>
 //   ctx == Return r
-//   ctx == dm_giio_bind (inst_io_cmds pi cmd arg) cont
-//   ctx == dm_giio_bind (eff_rc x) (fun eff_rc' -> dm_giio_bind cont1 (fun y -> dm_giio_bind (eff_rc' y) cont2)
+//   ctx == dm_gmio_bind (inst_io_cmds pi cmd arg) cont
+//   ctx == dm_gmio_bind (eff_rc x) (fun eff_rc' -> dm_gmio_bind cont1 (fun y -> dm_gmio_bind (eff_rc' y) cont2)
 // with that, one can do induction on the ctx to prove the non-interference
 // there is no axiom/law for erased
 // pi is Tot, it does not matter that it is erased
 //
 
-(**** Types using the giio directly **)
+(**** Types using the gmio directly **)
 
-type giio_typ_cmds (fl:erased tflag) (pi:monitorable_prop) =
+type gmio_acts (fl:erased tflag) (pi:policy_spec) (caller:bool) =
   (cmd : io_cmds) ->
   (arg : io_sig.args cmd) ->
-  dm_giio (io_resm cmd arg) fl
-    (to_hist 
-        (fun _ -> True)
-	(fun h r lt ->
-          enforced_locally pi h lt /\
-          (match r with
-          | Inr Contract_failure -> lt == []
-          | r' -> lt == [convert_call_to_event cmd arg r'])))
+  dm_gmio (io_resm cmd arg) fl
+    (to_hist (fun _ -> True)
+      (fun h r lt ->
+        enforced_locally pi h lt /\
+        (match r with
+        | Inr Contract_failure -> lt == []
+        | r' -> lt == [convert_call_to_event caller cmd arg r'])))
 
-val giio_inst_cmds : pi:monitorable_prop -> Tot (giio_typ_cmds AllActions pi)
-let giio_inst_cmds pi cmd arg =
-  _tot_reify_IIOwp (fun () -> inst_io_cmds pi cmd arg)
+val gmio_inst_cmds : #pi:policy_spec -> phi:policy pi -> Tot (gmio_acts AllActions pi false)
+let gmio_inst_cmds phi cmd arg =
+  _tot_reify_MIOwp (fun () -> inst_io_cmds phi cmd arg)
 
 // Binary parametricity for contexts, picking the trivial relation for erased.
 // It says that all contexts are parametric.
 
-let giio_eff_rc_typ_cont_wp (fl:erased tflag) (#t1:Type u#a) (#t2:Type u#b) (rc:rc_typ t1 t2) (x:t1) (y:t2) (initial_h:erased trace) =
+let gmio_eff_rc_typ_cont_wp (fl:erased tflag) (#t1:Type u#a) (#t2:Type u#b) (rc:rc_typ t1 t2) (x:t1) (y:t2) (initial_h:erased trace) =
   to_hist
     (fun h -> initial_h `suffix_of` h)
     (eff_rc_typ_cont_post rc initial_h x y)
 
-type giio_eff_rc_typ_cont (fl:erased tflag) (t1:Type u#a) (t2:Type u#b) (rc:rc_typ t1 t2) (x:t1) (initial_h:erased trace) =
-  y:t2 -> (dm_giio bool fl (giio_eff_rc_typ_cont_wp fl rc x y initial_h))
+type gmio_eff_rc_typ_cont (fl:erased tflag) (t1:Type u#a) (t2:Type u#b) (rc:rc_typ t1 t2) (x:t1) (initial_h:erased trace) =
+  y:t2 -> (dm_gmio bool fl (gmio_eff_rc_typ_cont_wp fl rc x y initial_h))
   
-type giio_eff_rc_typ (fl:erased tflag) (#t1 #t2:Type) (rc:rc_typ t1 t2) =
-  x:t1 -> (dm_giio (initial_h:(erased trace) & giio_eff_rc_typ_cont fl t1 t2 rc x initial_h) fl (to_hist (fun _ -> True) (fun h (| initial_h, _ |) lt -> h == reveal initial_h /\ lt == [])))
+type gmio_eff_rc_typ (fl:erased tflag) (#t1 #t2:Type) (rc:rc_typ t1 t2) =
+  x:t1 -> (dm_gmio (initial_h:(erased trace) & gmio_eff_rc_typ_cont fl t1 t2 rc x initial_h) fl (to_hist (fun _ -> True) (fun h (| initial_h, _ |) lt -> h == reveal initial_h /\ lt == [])))
 
 #set-options "--print_effect_args"
 
-val reify_eff_rc_cont : #fl:erased tflag -> #t1:Type -> #t2:Type -> #rc:rc_typ t1 t2 -> x:t1 -> initial_h:erased trace -> eff_rc_typ_cont fl t1 t2 rc x initial_h -> giio_eff_rc_typ_cont fl t1 t2 rc x initial_h
+val reify_eff_rc_cont : #fl:erased tflag -> #t1:Type -> #t2:Type -> #rc:rc_typ t1 t2 -> x:t1 -> initial_h:erased trace -> eff_rc_typ_cont fl t1 t2 rc x initial_h -> gmio_eff_rc_typ_cont fl t1 t2 rc x initial_h
 let reify_eff_rc_cont #fl #t1 #t2 #rc x initial_h cont (y:t2) =
-  _tot_reify_IIOwp (fun () -> cont y)
+  _tot_reify_MIOwp (fun () -> cont y)
 
-val reify_eff_rc : #fl:erased tflag -> #t1:Type -> #t2:Type -> #rc:rc_typ t1 t2 -> eff_rc_typ fl rc -> giio_eff_rc_typ fl rc
+val reify_eff_rc : #fl:erased tflag -> #t1:Type -> #t2:Type -> #rc:rc_typ t1 t2 -> eff_rc_typ fl rc -> gmio_eff_rc_typ fl rc
 let reify_eff_rc #fl #t1 #t2 #rc eff_rc x =
   admit ();
-  dm_giio_bind
+  dm_gmio_bind
     (initial_h:(erased trace) & eff_rc_typ_cont fl t1 t2 rc x initial_h)
-    (initial_h:(erased trace) & giio_eff_rc_typ_cont fl t1 t2 rc x initial_h)
+    (initial_h:(erased trace) & gmio_eff_rc_typ_cont fl t1 t2 rc x initial_h)
     fl NoActions
     (to_hist (fun _ -> True) (fun h (| initial_h, _ |) lt -> h == reveal initial_h /\ lt == []))
     (fun (| h, cont |) -> hist_return (| h, reify_eff_rc_cont x h cont |))
-    (_tot_reify_IIOwp (fun () -> eff_rc x))
-    (fun (| h, cont |) -> dm_giio_return _ (| h, reify_eff_rc_cont x h cont |))
+    (_tot_reify_MIOwp (fun () -> eff_rc x))
+    (fun (| h, cont |) -> dm_gmio_return _ (| h, reify_eff_rc_cont x h cont |))
 
-type giio_pck_eff_rc (fl:erased tflag) = pck:pck_rc & giio_eff_rc_typ fl (Mkdtuple3?._3 pck)
+type gmio_pck_eff_rc (fl:erased tflag) = pck:pck_rc & gmio_eff_rc_typ fl (Mkdtuple3?._3 pck)
 
-type giio_typ_eff_rcs (fl:erased tflag) (rcs:tree pck_rc) = 
-  eff_rcs:(tree (giio_pck_eff_rc fl)){
+type gmio_typ_eff_rcs (fl:erased tflag) (rcs:tree pck_rc) = 
+  eff_rcs:(tree (gmio_pck_eff_rc fl)){
     equal_trees rcs (map_tree eff_rcs dfst)}
 
-type giio_ctx (rc:rc_typ unit int) =
-  fl:erased tflag -> pi:erased monitorable_prop -> giio_typ_cmds fl pi -> giio_typ_eff_rcs fl (make_rc_tree rc) -> unit -> dm_giio int fl (to_hist (fun _ -> True) (fun _ _ _ -> True))
+type gmio_ctx (rc:rc_typ unit int) =
+  fl:erased tflag -> pi:erased policy_spec -> gmio_acts fl pi -> gmio_typ_eff_rcs fl (make_rc_tree rc) -> unit -> dm_gmio int fl (to_hist (fun _ -> True) (fun _ _ _ -> True))
 
 val bind1  : 
   #a: Type ->
   #b: Type ->
-  v: dm_giio a AllActions trivial_hist ->
-  f: (x: a -> dm_giio b AllActions trivial_hist) ->
-  Tot (dm_giio b AllActions trivial_hist)
-let bind1 #a #b = dm_giio_bind a b AllActions AllActions trivial_hist (fun _ -> trivial_hist)
+  v: dm_gmio a AllActions trivial_hist ->
+  f: (x: a -> dm_gmio b AllActions trivial_hist) ->
+  Tot (dm_gmio b AllActions trivial_hist)
+let bind1 #a #b = dm_gmio_bind a b AllActions AllActions trivial_hist (fun _ -> trivial_hist)
 
 let third
-  (eff_rc:giio_eff_rc_typ AllActions #'a #'b 'rc)
-  (cont1:dm_giio 'b AllActions trivial_hist)
-  (cont2: _ -> dm_giio 'c AllActions trivial_hist) 
+  (eff_rc:gmio_eff_rc_typ AllActions #'a #'b 'rc)
+  (cont1:dm_gmio 'b AllActions trivial_hist)
+  (cont2: _ -> dm_gmio 'c AllActions trivial_hist) 
   x :
-  dm_giio 'c AllActions trivial_hist =
+  dm_gmio 'c AllActions trivial_hist =
   admit ();
-  dm_giio_subcomp 'c AllActions AllActions _ trivial_hist (
-    dm_giio_bind 
-      (initial_h:(erased trace) & giio_eff_rc_typ_cont AllActions 'a 'b 'rc x initial_h)
+  dm_gmio_subcomp 'c AllActions AllActions _ trivial_hist (
+    dm_gmio_bind 
+      (initial_h:(erased trace) & gmio_eff_rc_typ_cont AllActions 'a 'b 'rc x initial_h)
       'c
       AllActions
       AllActions
       trivial_hist
-      (fun (| initial_h, _ |) -> hist_bind trivial_hist (fun y -> hist_bind (giio_eff_rc_typ_cont_wp AllActions 'rc x y initial_h) (fun _ -> trivial_hist)))
+      (fun (| initial_h, _ |) -> hist_bind trivial_hist (fun y -> hist_bind (gmio_eff_rc_typ_cont_wp AllActions 'rc x y initial_h) (fun _ -> trivial_hist)))
       (eff_rc x) 
       (fun (| initial_h, eff_rc' |) -> 
-        dm_giio_bind _ _ _ _ trivial_hist (fun y -> hist_bind (giio_eff_rc_typ_cont_wp AllActions 'rc x y initial_h) (fun _ -> trivial_hist))
+        dm_gmio_bind _ _ _ _ trivial_hist (fun y -> hist_bind (gmio_eff_rc_typ_cont_wp AllActions 'rc x y initial_h) (fun _ -> trivial_hist))
           cont1 
 	  (fun y -> 
-	    dm_giio_bind _ _ _ _ (giio_eff_rc_typ_cont_wp AllActions 'rc x y initial_h) (fun _ -> trivial_hist)
+	    dm_gmio_bind _ _ _ _ (gmio_eff_rc_typ_cont_wp AllActions 'rc x y initial_h) (fun _ -> trivial_hist)
 	      (eff_rc' y) 
 	      cont2)))
 
 let rec only_pi_and_rc
-  (pi:monitorable_prop)
-  (giio_cmds:giio_typ_cmds AllActions pi)
-  (eff_rc:giio_eff_rc_typ AllActions #'a #'b 'rc)
-  (m:dm_giio 'c AllActions trivial_hist) :
+  (pi:policy_spec)
+  (gmio_cmds:gmio_acts AllActions pi)
+  (eff_rc:gmio_eff_rc_typ AllActions #'a #'b 'rc)
+  (m:dm_gmio 'c AllActions trivial_hist) :
   GTot Type0 (decreases m) =
   (exists r. m == Return r) 
   \/
-  (exists cmd arg (cont:io_resm cmd arg -> dm_giio 'c AllActions trivial_hist).
-    (forall r.  (cont r) << m /\ only_pi_and_rc pi giio_cmds eff_rc (cont r)) ==>
-    (m == (bind1 (giio_cmds cmd arg) cont)))
+  (exists cmd arg (cont:io_resm cmd arg -> dm_gmio 'c AllActions trivial_hist).
+    (forall r.  (cont r) << m /\ only_pi_and_rc pi gmio_cmds eff_rc (cont r)) ==>
+    (m == (bind1 (gmio_cmds cmd arg) cont)))
   \/
-  (exists x (cont1:dm_giio 'b AllActions trivial_hist) (cont2: _ -> dm_giio 'c AllActions trivial_hist). 
-    ((cont1 << m /\ only_pi_and_rc pi giio_cmds eff_rc cont1) /\
-    (forall r. (cont2 r) << m /\ only_pi_and_rc pi giio_cmds eff_rc (cont2 r))) ==> 
+  (exists x (cont1:dm_gmio 'b AllActions trivial_hist) (cont2: _ -> dm_gmio 'c AllActions trivial_hist). 
+    ((cont1 << m /\ only_pi_and_rc pi gmio_cmds eff_rc cont1) /\
+    (forall r. (cont2 r) << m /\ only_pi_and_rc pi gmio_cmds eff_rc (cont2 r))) ==> 
     m == third eff_rc cont1 cont2 x)
 
 (** *** Effect polymorphism *)
@@ -234,30 +234,30 @@ noeq type monad = {
   (* We don't want acts to be part of this monad because we want to provide different versions *)
 }
 
-let dm_giio' (fl:erased tflag) (pi:monitorable_prop) (a:Type) = dm_giio a fl (pi_as_hist pi)
+let dm_gmio' (fl:erased tflag) (pi:policy_spec) (a:Type) = dm_gmio a fl (pi_as_hist pi)
 
-let as_giio_dm (w:dm_giio' 'f 'p 'a) : dm_giio 'a 'f (pi_as_hist 'p) = 
-  let tree : iio 'a = w in
-  assert (pi_as_hist 'p `Hist.hist_ord` IIO.dm_giio_theta tree);
+let as_gmio_dm (w:dm_gmio' 'f 'p 'a) : dm_gmio 'a 'f (pi_as_hist 'p) = 
+  let tree : mio 'a = w in
+  assert (pi_as_hist 'p `Hist.hist_ord` MIO.dm_gmio_theta tree);
   tree
 
-let as_giio_dm' (w:dm_giio 'a 'f (pi_as_hist 'p)) : dm_giio' 'f 'p 'a = w
+let as_gmio_dm' (w:dm_gmio 'a 'f (pi_as_hist 'p)) : dm_gmio' 'f 'p 'a = w
 
-let lemma_bind_pi_implies_pi (#a #b:Type) (pi:monitorable_prop) : 
+let lemma_bind_pi_implies_pi (#a #b:Type) (pi:policy_spec) : 
   Lemma (pi_as_hist #b pi `hist_ord` (hist_bind (pi_as_hist #a pi) (fun (_:a) -> pi_as_hist pi))) = admit ()
 
-let dm_giio_return' (a:Type) (fl:erased tflag) (x:a) : dm_giio a fl (hist_return x) by (compute ()) =
-  dm_iio_return a x
+let dm_gmio_return' (a:Type) (fl:erased tflag) (x:a) : dm_gmio a fl (hist_return x) by (compute ()) =
+  dm_mio_return a x
 
-let dm_mon (fl:erased tflag) (pi:monitorable_prop) : monad = {
-  m = dm_giio' fl pi;
-  ret = (fun (x:'a) -> dm_giio_return' 'a fl x);
-  bind = (fun (m:dm_giio' fl pi 'a) (k:'a -> dm_giio' fl pi 'b) -> 
+let dm_mon (fl:erased tflag) (pi:policy_spec) : monad = {
+  m = dm_gmio' fl pi;
+  ret = (fun (x:'a) -> dm_gmio_return' 'a fl x);
+  bind = (fun (m:dm_gmio' fl pi 'a) (k:'a -> dm_gmio' fl pi 'b) -> 
     let wp : Hist.hist 'b = Hist.hist_bind (pi_as_hist #'a pi) (fun _ -> pi_as_hist pi) in 
-    let tr : dm_giio 'b fl wp = dm_giio_bind _ _ _ _ _ _ (as_giio_dm m) (fun x -> as_giio_dm (k x)) in
+    let tr : dm_gmio 'b fl wp = dm_gmio_bind _ _ _ _ _ _ (as_gmio_dm m) (fun x -> as_gmio_dm (k x)) in
     lemma_bind_pi_implies_pi #'a #'b pi;
-    let w = dm_giio_subcomp 'b _ _ wp (pi_as_hist pi) tr in
-    as_giio_dm' w)
+    let w = dm_gmio_subcomp 'b _ _ wp (pi_as_hist pi) tr in
+    as_gmio_dm' w)
 }
 
 type effpoly_rc (mon:monad) = (unit -> mon.m (int -> mon.m (Universe.raise_t (bool <: Type))))
@@ -268,7 +268,7 @@ type effpoly_ctx =
 #set-options "--print_universes"
 
 (**
-val law : rc:rc_typ unit int -> effpoly_ctx -> giio_ctx rc
+val law : rc:rc_typ unit int -> effpoly_ctx -> gmio_ctx rc
 let law rc effctx fl pi io_acts effrc =
   effctx (dm_mon fl pi) io_acts
 **)
@@ -276,11 +276,11 @@ let law rc effctx fl pi io_acts effrc =
 (** *** Parametricity **)
 // Type of contexts
 let ctx_type rc =
-  fl:erased tflag -> pi:erased monitorable_prop -> typ_io_cmds fl pi -> typ_eff_rcs fl (make_rc_tree rc) -> unit -> dm_giio int fl (to_hist (fun _ -> True) (fun _ _ _ -> True))
+  fl:erased tflag -> pi:erased policy_spec -> typ_io_cmds fl pi -> typ_eff_rcs fl (make_rc_tree rc) -> unit -> dm_gmio int fl (to_hist (fun _ -> True) (fun _ _ _ -> True))
 
 assume val typ_io_cmds_r :
   fl0: erased tflag -> fl1: erased tflag -> // erased_r is trivial
-  pi0: erased monitorable_prop -> pi1: erased monitorable_prop ->
+  pi0: erased policy_spec -> pi1: erased policy_spec ->
   io0: typ_io_cmds fl0 pi0 -> io1: typ_io_cmds fl1 pi1 ->
   Type0
 // let typ_io_cmds_r fl0 fl1 pi0 pi1 io0 io1 = io0 == io1
@@ -298,14 +298,14 @@ assume val typ_eff_rcs_r :
 // Relation of contexts (it cannot type check because of the effect, but would the monad be enough?)
 let ctx_type_r rc (ctx0 ctx1 : ctx_type rc) =
   fl0: erased tflag -> fl1: erased tflag -> // erased_r is trivial
-  pi0: erased monitorable_prop -> pi1: erased monitorable_prop ->
+  pi0: erased policy_spec -> pi1: erased policy_spec ->
   io0: typ_io_cmds fl0 pi0 -> io1: typ_io_cmds fl1 pi1 ->
   ior: typ_io_cmds_r fl0 fl1 pi0 pi1 io0 io1 ->
   t0: typ_eff_rcs fl0 (make_rc_tree rc) ->
   t1: typ_eff_rcs fl1 (make_rc_tree rc) ->
   tr: typ_eff_rcs_r _ fl0 fl1 t0 t1 ->
   // ignoring unit
-  // Assuming the relation on dm_giio is equality
+  // Assuming the relation on dm_gmio is equality
   Lemma (ctx0 fl0 pi0 io0 t0 () == ctx1 fl1 pi1 io1 t1 ())
 
 // typ_io_cmds NoAction = Inr Contract_failure
@@ -321,25 +321,25 @@ assume val ctx_param :
 val bind1  : 
   #a: Type ->
   #b: Type ->
-  v: dm_giio a AllActions trivial_hist ->
-  f: (x: a -> dm_giio b AllActions trivial_hist) ->
-  Tot (dm_giio b AllActions trivial_hist)
-let bind1 #a #b = dm_giio_bind a b AllActions AllActions trivial_hist (fun _ -> trivial_hist)
+  v: dm_gmio a AllActions trivial_hist ->
+  f: (x: a -> dm_gmio b AllActions trivial_hist) ->
+  Tot (dm_gmio b AllActions trivial_hist)
+let bind1 #a #b = dm_gmio_bind a b AllActions AllActions trivial_hist (fun _ -> trivial_hist)
 
-let rec only_pi_and_rc (pi:monitorable_prop) (eff_rc:eff_rc_typ AllActions #'a #'b 'rc) (m:dm_giio 'c AllActions trivial_hist) : GTot Type0 (decreases m) =
+let rec only_pi_and_rc (pi:policy_spec) (eff_rc:eff_rc_typ AllActions #'a #'b 'rc) (m:dm_gmio 'c AllActions trivial_hist) : GTot Type0 (decreases m) =
   
   (exists r. m == Return r) 
   \/
-  (exists cmd arg (cont:io_resm cmd arg -> dm_giio 'c AllActions trivial_hist).
+  (exists cmd arg (cont:io_resm cmd arg -> dm_gmio 'c AllActions trivial_hist).
     (forall r.  (cont r) << m /\ only_pi_and_rc pi eff_rc (cont r)) ==>
-    (m == (bind1 (__reify_IIOwp (fun () -> inst_io_cmds pi cmd arg <: IIOwp (io_resm cmd arg) AllActions trivial_hist)) cont)))
+    (m == (bind1 (__reify_MIOwp (fun () -> inst_io_cmds pi cmd arg <: MIOwp (io_resm cmd arg) AllActions trivial_hist)) cont)))
   \/
-  (exists x (cont1:dm_giio 'b AllActions trivial_hist) (cont2: _ -> dm_giio 'c AllActions trivial_hist). 
+  (exists x (cont1:dm_gmio 'b AllActions trivial_hist) (cont2: _ -> dm_gmio 'c AllActions trivial_hist). 
     ((cont1 << m /\ only_pi_and_rc pi eff_rc cont1) /\
     (forall r. (cont2 r) << m /\ only_pi_and_rc pi eff_rc (cont2 r))) ==> 
-    m == dm_giio_bind _ _ AllActions AllActions _ _ (__reify_IIOwp (fun () -> eff_rc x)) (fun (| _, eff_rc' |) -> 
+    m == dm_gmio_bind _ _ AllActions AllActions _ _ (__reify_MIOwp (fun () -> eff_rc x)) (fun (| _, eff_rc' |) -> 
                bind1 cont1 (fun y -> 
-                 bind1 (__reify_IIOwp (fun () -> eff_rc' y)) cont2)))
+                 bind1 (__reify_MIOwp (fun () -> eff_rc' y)) cont2)))
 *)  
 
 let ni pi rc ctx = admit ()
@@ -364,7 +364,7 @@ about whole/partial source programs. **)
 
 (** Whole programs **)
 
-let read_content (fnm:string) : IIO (r:(resexn string){~(r == Inr Contract_failure)}) IOActions
+let read_content (fnm:string) : MIO (r:(resexn string){~(r == Inr Contract_failure)}) IOActions
   (requires (fun _ -> True))
   (ensures (fun _ r lt -> 
     (Inr? r /\ lt == [EOpenfile fnm (Inr (Inr?.v r))]) \/
@@ -374,14 +374,14 @@ let read_content (fnm:string) : IIO (r:(resexn string){~(r == Inr Contract_failu
   | Inl fd -> static_cmd Read fd
   | Inr err -> Inr err
 
-let rec get_fd_content (fd:file_descr) (t:IIO.Sig.trace) : option string =
+let rec get_fd_content (fd:file_descr) (t:MIO.Sig.trace) : option string =
   match t with
   | [] -> None
   | (ERead fd' (Inl msg')) :: tl -> if fd = fd' then (Some msg') else (get_fd_content fd tl)
   | (ERead fd' (Inr msg')) :: tl -> if fd = fd' then None else (get_fd_content fd tl)
   | _ :: tl -> get_fd_content fd tl
   
-let rec get_content (fnm:string) (t:IIO.Sig.trace) : option string =
+let rec get_content (fnm:string) (t:MIO.Sig.trace) : option string =
   match t with
   | [] -> None
   | (EOpenfile fnm' (Inl fd')) :: tl -> if fnm = fnm' then (get_fd_content fd' tl) else (get_content fnm tl)
@@ -405,7 +405,7 @@ val hyperprop_tp1 : unit ->  Lemma (
     get_content "config.txt" t1 == get_content "config.txt" t2 ==> r1 == r2)))
 let hyperprop_tp1 () = ()
 
-let whole1 () : IIO int AllActions 
+let whole1 () : MIO int AllActions 
   (requires (fun _ -> True))
   (ensures (fun _ r lt -> tp1 (Finite_trace lt r))) =
   let config = read_content "config.txt" in
@@ -447,7 +447,7 @@ let hyperprop_whole1 () =
    - [ ] is it the theorem we want?
    - [ ] can we write it in a more simple way to be easier to prove in F*?
    - [ ] prove *)
-val leak_the_same : trace -> trace -> pi:monitorable_prop -> rc:('a -> trace -> 'b -> trace -> bool) -> Type0
+val leak_the_same : trace -> trace -> pi:policy_spec -> rc:('a -> trace -> 'b -> trace -> bool) -> Type0
 let leak_the_same h1 h2 pi rc =
   // for each valid local trace of h1,
   // there exists a valid local trace for h2
@@ -459,11 +459,11 @@ let leak_the_same h1 h2 pi rc =
       (forall arg res. rc arg h1 res lt1 == rc arg h2 res lt2)))
 
 val tini : 
-  pi : monitorable_prop ->
+  pi : policy_spec ->
   (** for any runtime check **)
   rc : ('a -> trace -> 'b -> trace -> bool) ->
   (** the ctx is in a first-order setting. I don't think it matters **)
-  ctx: (fl:erased tflag -> pi:erased monitorable_prop -> typ_io_cmds fl pi -> typ_eff_rcs fl (make_rc_tree rc) -> unit -> IIO int fl (fun _ -> True) (fun _ _ _ -> True)) ->
+  ctx: (fl:erased tflag -> pi:erased policy_spec -> typ_io_cmds fl pi -> typ_eff_rcs fl (make_rc_tree rc) -> unit -> MIO int fl (fun _ -> True) (fun _ _ _ -> True)) ->
   Lemma (
                                   (** one has to instantiate the ctx to be able to call beh **)
     let bh = beh_ctx #(fun _ -> True) (ctx AllActions pi (inst_io_cmds pi) (make_rcs_eff (make_rc_tree rc))) in
@@ -497,11 +497,11 @@ let tini pi rc ctx = admit ()
    We do NOT want this theorem, because this is for nondeterministic programs,
    while our programs are determinstic, thus this is too complex! *)
 val gni : 
-  pi : monitorable_prop ->
+  pi : policy_spec ->
   (** for any runtime check **)
   rc : ('a -> trace -> 'b -> trace -> bool) ->
   (** the ctx is in a first-order setting. I don't think it matters **)
-  ctx: (fl:erased tflag -> pi:erased monitorable_prop -> typ_io_cmds fl pi -> typ_eff_rcs fl (make_rc_tree rc) -> unit -> IIO int fl (fun _ -> True) (fun _ _ _ -> True)) ->
+  ctx: (fl:erased tflag -> pi:erased policy_spec -> typ_io_cmds fl pi -> typ_eff_rcs fl (make_rc_tree rc) -> unit -> MIO int fl (fun _ -> True) (fun _ _ _ -> True)) ->
   Lemma (
     let eff_rcs = make_rcs_eff (make_rc_tree rc) in
     let bh = beh_ctx #(fun _ -> True) (ctx AllActions pi (inst_io_cmds pi) eff_rcs) in
@@ -540,7 +540,7 @@ val gni0 :
     * ctx should also take instrumented actions
     * ctx should also take the contracts *)
 val gni_v0 : 
-  ctx:(fl:erased tflag -> unit -> IIO int fl (fun _ -> True) (fun _ _ _ -> True)) ->
+  ctx:(fl:erased tflag -> unit -> MIO int fl (fun _ -> True) (fun _ _ _ -> True)) ->
   Lemma (
     let bh = beh_ctx #(fun _ -> True) (ctx AllActions) in
     forall t1 t2. t1 `pt_mem` bh /\ t2 `pt_mem` bh ==>
@@ -551,7 +551,7 @@ val gni_v0 :
              
 let gni_v0 ctx =
   let bh = beh_ctx #(fun _ -> True) (ctx AllActions) in
-  let reified_ctx : dm_giio int AllActions (to_hist (fun _ -> True) (fun _ _ _ -> True)) = __reify_IIOwp (ctx AllActions) in
+  let reified_ctx : dm_gmio int AllActions (to_hist (fun _ -> True) (fun _ _ _ -> True)) = __reify_MIOwp (ctx AllActions) in
   introduce forall t1 t2.
   t1 `pt_mem` bh /\ t2 `pt_mem` bh 
   ==> (exists t3. t3 `pt_mem` bh /\ fst t1 == fst t3 /\ snd t2 == snd t3) 
@@ -562,8 +562,8 @@ let gni_v0 ctx =
       let newH = (fst t1) in
       let t3 = (newH, snd t2) in 
       assert (t2 `pt_mem` bh); (** unfolds to: **)
-      //assert ((snd t2) `member_of #event` beh_giio reified_ctx (fst t2)); (* not sure why it does not work *)
-      assume ((snd t2) `member_of` beh_giio reified_ctx newH); (** folds into: **)
+      //assert ((snd t2) `member_of #event` beh_gmio reified_ctx (fst t2)); (* not sure why it does not work *)
+      assume ((snd t2) `member_of` beh_gmio reified_ctx newH); (** folds into: **)
       assert (t3 `pt_mem` bh) by (
         binder_retype (nth_binder (-1)); norm [delta_only [`%member_of];iota]; trefl ();
         norm [delta_only [`%pt_mem;`%beh_ctx;`%_beh_ctx]; iota]; 
@@ -576,8 +576,8 @@ let gni_v0 ctx =
 
 val pprog1 : 
   fl:erased tflag ->
-  ctx:(unit -> IIO int fl (fun _ -> True) (fun _ _ _ -> True)) ->
-  IIO int (fl + IOActions) (fun _ -> True) (fun _ _ _ -> True) 
+  ctx:(unit -> MIO int fl (fun _ -> True) (fun _ _ _ -> True)) ->
+  MIO int (fl + IOActions) (fun _ -> True) (fun _ _ _ -> True) 
 let pprog1 fl ctx =
   let msg = read_content "secrets.txt" in  
  // let _ = ctx () in
@@ -596,13 +596,13 @@ val hyperprop_pprog1 : ctx:_ -> tr1:_ -> tr2:_ ->
        | _, _ -> False))
 
 let hyperprop_pprog1 ctx tr1 tr2 =
-  let bh = beh_giio (__reify_IIOwp ((fun () -> pprog1 AllActions ctx))) [] in
+  let bh = beh_gmio (__reify_MIOwp ((fun () -> pprog1 AllActions ctx))) [] in
  // reveal_opaque (`%beh) beh;
  // assert (beh ws == bh); 
   match tr1, tr2 with
   | Finite_trace t1 r1, Finite_trace t2 r2 -> begin
     assert (Finite_trace t1 r1 `member_of` bh ==> r1 == 7) by (
-      norm [delta_only [`%beh;`%member_of;`%beh_giio];iota];
+      norm [delta_only [`%beh;`%member_of;`%beh_gmio];iota];
       //norm [delta_only [`%link1;`%pprog1];iota];
      dump "H");
     admit ();
